refactor to not use Finset in seq

Pom/Lpo/Operations/Seq/Branches.lean
@@ -22,50 +22,44 @@ lemma stuck_antitone : @Antitone (Lpofin l) _ _ _ stuck := by
     exact hform
 
 -- A node is in the exntensible set if it is possible for it not be stuck
-open Classical in
-noncomputable def extens (α : Lpofin l) : Finset Node :=
-  α.nodes_finset.filter fun x ↦ ¬ α.form x ≤ α.stuck
+def extens (α : Lpofin l) : Set Node :=
+  { x ∈ α.nodes | ¬ α.form x ≤ α.stuck }
+
+lemma extens_finite (α : Lpofin l) : α.extens.Finite := by
+  apply α.property.subset; intro x hx; exact hx.1
 
 lemma extens_not_bot {α : Lpofin l} {x : Node} : x ∈ α.extens → α.lab x ≠ ⊥ := by
-  intro h; simp only [extens, Finset.mem_filter] at h; intro heq; apply h.2; intro v hform
+  intro h heq; apply h.2; intro v hform
   refine ⟨⟨x, ?_, heq⟩, hform⟩
   exact (α.val.property.form_dom x).mp ⟨v, hform⟩
 
-open Classical in
-lemma extens_subset_nodes {α : Lpofin l} : ∀ x ∈ α.extens, x ∈ α.nodes := by
-  intro x hx; exact (Set.Finite.mem_toFinset _).mp (Finset.mem_filter.mp hx).1
-
 lemma extens_monotone : @Monotone (Lpofin l) _ _ _ extens := by
-  intro α β hle x; simp only [extens, Finset.mem_filter, and_imp]; intro hx hstuck
-  have hx' := (Set.Finite.mem_toFinset _).mp hx
-  refine ⟨(Set.Finite.mem_toFinset _).mpr (hle.nodes hx'), fun hc ↦ ?_⟩
+  intro α β hle x ⟨hx, hstuck⟩
+  refine ⟨hle.nodes hx, ?_⟩; intro hc
   refine hstuck (fun v hform ↦ stuck_antitone hle v (hc v ?_))
-  simp only [form]; rw [← hle.form x hx']; exact hform
+  simp only [form]; rw [← hle.form x hx]; exact hform
 
-open Classical in
 lemma le_extens {α β : Lpofin l} (hle : α ≤ β) :
-    α.extens = β.extens.filter fun x ↦ ¬ (β.form x ≤ α.stuck) := by
+    α.extens = { x ∈ β.extens | ¬ (β.form x ≤ α.stuck) } := by
   ext x; constructor
-  · intro hx; refine Finset.mem_filter.mpr ⟨extens_monotone hle hx, ?_⟩
-    intro c; refine (Finset.mem_filter.mp hx).2 (le_trans ?_ c)
+  · intro hx; refine ⟨extens_monotone hle hx, ?_⟩
+    intro c; refine hx.2 (le_trans ?_ c)
     exact le_form hle
-  · intro hx; obtain ⟨hx, hstk⟩ := Finset.mem_filter.mp hx
-    obtain ⟨hx', _⟩ := Finset.mem_filter.mp hx
-    apply (Set.Finite.mem_toFinset _).mp at hx'
-    rcases hle.succ _  hx' with hxα | ⟨y, ⟨hy, hbot⟩, hyx⟩
-    · refine Finset.mem_filter.mpr ⟨(Set.Finite.mem_toFinset _).mpr hxα, ?_⟩
+  · intro ⟨⟨hx, _⟩, hstk⟩
+    rcases hle.succ _  hx with hxα | ⟨y, ⟨hy, hbot⟩, hyx⟩
+    · refine ⟨hxα, ?_⟩
       intro c; refine hstk (le_of_eq_of_le (Eq.symm ?_) c)
       exact hle.form _ hxα
     · exfalso; refine hstk (((β.val.property.form y (hle.nodes hy)).2 _ hyx).trans ?_)
       refine le_of_eq_of_le (Eq.symm (hle.form _ hy)) ?_
       intro v hform; exact ⟨⟨y, hy, hbot⟩, hform⟩
 
-def conj (α : Lpofin l) (S : Finset Node) : Form Node :=
+def conj (α : Lpofin l) (S : Set Node) : Form Node :=
   Form.sAnd fun x : ↑S ↦ α.form x.val
 
-def branches_set (α : Lpofin l) : Set (Form Node) :=
+def branches (α : Lpofin l) : Set (Form Node) :=
   α.conj ''
-  { S : Finset Node
+  { S : Set Node
   | S.Nonempty ∧
     S ⊆ α.extens ∧
     (α.conj S).sat ∧
@@ -73,67 +67,58 @@ def branches_set (α : Lpofin l) : Set (Form Node) :=
     ∀ T, S ⊂ T → T ⊆ α.extens → ¬ Form.sat (fun v ↦ ∀ x ∈ T, α.form x v)
   }
 
-lemma branches_finite (α : Lpofin l) : α.branches_set.Finite := by
+lemma branches_finite (α : Lpofin l) : α.branches.Finite := by
   refine Set.Finite.image _ ?_
-  refine Set.Finite.subset α.extens.powerset.finite_toSet ?_
-  intro s ⟨_, hsub, _⟩; simp only [Finset.coe_powerset, Set.mem_preimage, Set.mem_powerset_iff,
-    Finset.coe_subset, hsub]
+  refine α.extens_finite.powerset.subset ?_
+  intro s ⟨_, hsub, _⟩; exact hsub
 
-noncomputable def branches (α : Lpofin l) : Finset (Form Node) := α.branches_finite.toFinset
-
-lemma branches_set_monotone : @Monotone (Lpofin l) _ _ _ branches_set := by
+lemma branches_monotone : @Monotone (Lpofin l) _ _ _ branches := by
   classical
   rintro α β hle φ ⟨S, ⟨hne, hsub, hsat, hstuck, hmax⟩, hφ⟩; subst hφ
   refine ⟨S, ⟨hne, ?_, ?_, ?_, ?_⟩, ?_⟩
   · exact le_trans hsub (extens_monotone hle)
   · rcases hsat with ⟨v, hv⟩; use v; intro x
     refine (congrFun (hle.form x ?_) _).mp (hv x)
-    have hx' := Finset.mem_of_mem_filter _ (hsub x.property)
-    exact (Set.Finite.mem_toFinset _).mp hx'
+    exact hsub x.property |>.1
   · intro v hform hstuck'; refine hstuck v ?_ ?_
     · intro x; refine (congr_fun (hle.form x ?_) v).mpr (hform x)
-      have hx' := Finset.mem_of_mem_filter _ (hsub x.property)
-      exact (Set.Finite.mem_toFinset _).mp hx'
+      exact hsub x.property |>.1
     · exact stuck_antitone hle v hstuck'
-  · intro T hST hT ⟨v, hc⟩; obtain ⟨x, hxT, hxS⟩ := Finset.exists_of_ssubset hST
+  · intro T hST hT ⟨v, hc⟩; obtain ⟨x, hxT, hxS⟩ := Set.exists_of_ssubset hST
     have hform : α.conj S v := by
       intro y; refine (congrFun (hle.form _ ?_) _).mpr (hc _ ?_)
-      · exact extens_subset_nodes _ (hsub y.property)
-      · exact (Finset.ssubset_def.mp hST).1 y.property
-    rcases hle.succ _ (extens_subset_nodes _ (hT hxT))
+      · exact (hsub y.property).1
+      · exact hST.subset y.property
+    rcases hle.succ _ (hT hxT).1
       with hx | ⟨y, hy, hyx⟩
-    · refine hmax (insert x S) (Finset.ssubset_insert hxS) ?_ ?_
-      · refine Finset.insert_subset (Finset.mem_filter.mpr ⟨?_, ?_⟩) hsub
-        · exact (Set.Finite.mem_toFinset _).mpr hx
+    · refine hmax (insert x S) (Set.ssubset_insert hxS) ?_ ?_
+      · refine Set.insert_subset ⟨hx, ?_⟩ hsub
         · intro c; refine hstuck v hform ?_
           exact c v ((congrFun (hle.form _ hx) _).mpr (hc _ hxT))
-      · use v; intro y hy; rcases Finset.mem_insert.mp hy with rfl | hy'
+      · use v; intro y hy; rcases Set.mem_insert_iff.mp hy with rfl | hy'
         · exact (congrFun (hle.form y hx) _).mpr (hc y hxT)
         · refine (congrFun (hle.form y ?_) _).mpr (hc y ?_)
-          · exact extens_subset_nodes _ (hsub hy')
-          · exact Finset.mem_of_subset (Finset.ssubset_def.mp hST).1 hy'
+          · exact (hsub hy').1
+          · exact hST.subset hy'
     · refine hstuck v hform ⟨⟨y, hy⟩, ?_⟩
       refine (congrFun (hle.form _ hy.1) _).mpr ?_
       exact (β.val.property.form _ (hle.nodes hy.1)).2 _ hyx v (hc _ hxT)
   · ext1 v; refine forall_congr fun x ↦ ?_; ext; constructor
     · intro h; refine (congr_fun (hle.form x ?_) v).mpr h
-      have hx' := Finset.mem_of_mem_filter _ (hsub x.property)
-      exact (Set.Finite.mem_toFinset _).mp hx'
+      exact (hsub x.property).1
     · intro h; refine (congr_fun (hle.form x ?_) v).mp h
-      have hx' := Finset.mem_of_mem_filter _ (hsub x.property)
-      exact (Set.Finite.mem_toFinset _).mp hx'
+      exact (hsub x.property).1
 
-lemma le_branches_set {α β : Lpofin l} (hle : α ≤ β) :
-    α.branches_set = { φ ∈ β.branches_set | φ ≤ α.stuck.not } := by
+lemma le_branches {α β : Lpofin l} (hle : α ≤ β) :
+    α.branches = { φ ∈ β.branches | φ ≤ α.stuck.not } := by
   ext φ; constructor
   · intro h; constructor
-    · exact branches_set_monotone hle h
+    · exact branches_monotone hle h
     · rcases h with ⟨_, ⟨_, _, _, hstuck, _⟩, rfl⟩
       exact hstuck
   · rintro ⟨⟨S, ⟨hne, hsub, ⟨v, hsat⟩, _, hmax⟩, rfl⟩, hstuck⟩
     have hS x (hx : x ∈ S) : x ∈ α.nodes := by
-      have hx' := extens_subset_nodes _ (hsub hx)
-      rcases hle.succ _ hx' with hxα | ⟨y, hbot, hyx⟩
+      rcases hle.succ _ (hsub hx).1 with hxα | ⟨y, hbot, hyx⟩
       · exact hxα
       · exfalso; refine forall_not_of_not_exists (hstuck v hsat) ⟨y, hbot⟩ ?_
         refine (congrFun (hle.form y hbot.1) _).mpr ?_
@@ -141,45 +126,39 @@ lemma le_branches_set {α β : Lpofin l} (hle : α ≤ β) :
         exact hsat ⟨_, hx⟩
     refine ⟨S, ⟨hne, ?_, ⟨v, ?_⟩, ?_, ?_⟩, ?_⟩
     · intro x hx; rw [le_extens hle]
-      classical refine Finset.mem_filter.mpr ⟨?_, ?_⟩
-      · exact hsub hx
-      · intro c; exact hstuck v hsat (c v (hsat ⟨x, hx⟩))
+      refine ⟨hsub hx, ?_⟩
+      intro c; exact hstuck v hsat (c v (hsat ⟨x, hx⟩))
     · intro x; exact (congrFun (hle.form x (hS _ x.property)) _).mpr (hsat x)
     · refine le_trans ?_ hstuck; intro u hu x
       exact (congrFun (hle.form _ (hS _ x.property)) _).mp (hu x)
     · intro T hST hT ⟨u, hu⟩; refine hmax T hST ?_ ?_
       · exact le_trans hT (extens_monotone hle)
       · use u; intro x hx; refine (congrFun (hle.form _ ?_) _).mp (hu _ hx)
-        exact extens_subset_nodes _ (hT hx)
+        exact (hT hx).1
     · ext1 u; refine forall_congr fun x ↦ ?_
       exact congrFun (hle.form x (hS _ x.property)) _
-
-lemma branches_monotone : @Monotone (Lpofin l) _ _ _ branches := by
-  unfold branches; intro α β hle
-  simp only [Finset.le_eq_subset, Set.Finite.subset_toFinset, Set.Finite.coe_toFinset]
-  exact branches_set_monotone hle
 
 lemma branches_not_mutually_sat {α : Lpofin l} {φ ψ : Form Node}
     (hφ : φ ∈ α.branches) (hψ : ψ ∈ α.branches) (hneq : φ ≠ ψ) :
     ∀ v, ¬ (φ v ∧ ψ v) := by
   intro v ⟨h₁, h₂⟩
-  rcases (Set.Finite.mem_toFinset _).mp hφ with ⟨S, ⟨_, hsub, _, _, hmax⟩, rfl⟩
-  rcases (Set.Finite.mem_toFinset _).mp hψ with ⟨T, ⟨_, hsub', _, _, hmax'⟩, rfl⟩
-  refine hmax (S ∪ T) ⟨Finset.subset_union_left, ?_⟩ ?_ ?_
+  obtain ⟨S, ⟨_, hsub, _, _, hmax⟩, rfl⟩ := hφ
+  obtain ⟨T, ⟨_, hsub', _, _, hmax'⟩, rfl⟩ := hψ
+  refine hmax (S ∪ T) ⟨Set.subset_union_left, ?_⟩ ?_ ?_
   · intro h; apply hneq; refine congrArg _ ?_; ext x; constructor
     · intro hx; by_contra ht; refine hmax' (insert x T) ?_ ?_ ?_
-      · exact Finset.ssubset_insert ht
-      · intro y hy; rcases Finset.mem_insert.mp hy with rfl | hy
+      · exact Set.ssubset_insert ht
+      · intro y hy; rcases Set.mem_insert_iff.mp hy with rfl | hy
         · exact hsub hx
         · exact hsub' hy
-      · use v; intro y hy; rcases Finset.mem_insert.mp hy with rfl | hy
+      · use v; intro y hy; rcases Set.mem_insert_iff.mp hy with rfl | hy
         · exact h₁ ⟨y, hx⟩
         · exact h₂ ⟨y, hy⟩
-    · intro hx; exact h (Finset.subset_union_right hx)
-  · intro x hx; rcases Finset.mem_union.mp hx with hx | hx
+    · intro hx; exact h (Set.subset_union_right hx)
+  · rintro x (hx | hx)
     · exact hsub hx
     · exact hsub' hx
-  · use v; intro x hx; rcases Finset.mem_union.mp hx with hx | hx
+  · use v; rintro x (hx | hx)
     · exact h₁ ⟨x, hx⟩
     · exact h₂ ⟨x, hx⟩
 
